examples/n_german/Symmetric.thy
@@ -1,0 +1,212 @@
+theory Symmetric
+  imports paraTheoryCmpzb
+begin
+
+
+subsection \<open>Rule set parameterized by processes\<close>
+
+text \<open>We consider a special form of rule set, where there is a set associated
+to each process i\<close>
+definition rulesOverDownN :: "nat \<Rightarrow> (nat \<Rightarrow> rule set) \<Rightarrow> rule set" where
+  "rulesOverDownN N f = {r. \<exists>n\<le>N. r \<in> f n}"
+
+text \<open>There is a general theorem for showing symmetry\<close>
+definition symmetricParamRules :: "nat \<Rightarrow> (nat \<Rightarrow> rule set) \<Rightarrow> bool" where
+  "symmetricParamRules N f = (\<forall>p i. p permutes {x. x \<le> N} \<longrightarrow> i \<le> N \<longrightarrow> applySym2Rule p ` f i = f (p i))"
+
+theorem symProtFromSymmetricParam:
+  assumes "symmetricParamRules N f"
+  shows "symProtRules N (rulesOverDownN N f)"
+proof -
+  have 1: "applySym2Rule p r \<in> f (p n)"
+    if "p permutes {x. x \<le> N}" "n \<le> N" "r \<in> f n" for p r n
+  proof -
+    have "applySym2Rule p ` f n = f (p n)"
+      using assms unfolding symmetricParamRules_def
+      using that(1,2) by auto
+    then show ?thesis
+      using that(3) by auto
+  qed
+  show ?thesis
+    unfolding symProtRules_def rulesOverDownN_def
+    apply auto
+    subgoal for p r n
+      apply (rule exI[where x="p n"])
+      apply auto
+      using permutes_in_image apply fastforce
+      using assms unfolding symmetricParamRules_def
+      using 1 by auto
+    done
+qed
+
+
+subsection \<open>Formula set parameterized by two processes\<close>
+
+text \<open>Likewise, we consider special cases of parameterized formulas.\<close>
+definition symmetricParamFormulas2 :: "nat \<Rightarrow> (nat \<Rightarrow> nat \<Rightarrow> formula) \<Rightarrow> bool" where
+  "symmetricParamFormulas2 N f =
+    (\<forall>p i j. p permutes {x. x \<le> N} \<longrightarrow> i \<le> N \<longrightarrow> j \<le> N \<longrightarrow> applySym2Form p (f i j) = f (p i) (p j))"
+
+definition formulasOverDownN2 :: "nat \<Rightarrow> (nat \<Rightarrow> nat \<Rightarrow> formula) \<Rightarrow> (nat \<Rightarrow> formula list)" where
+  "formulasOverDownN2 N f i = map (f i) (down N)"
+
+lemma set_down: "set (down N) = {x. x \<le> N}"
+  apply (induction N)
+   apply auto[1] by fastforce
+
+lemma symParamFormulas:
+  assumes "symmetricParamFormulas2 N f"
+    and "p permutes {x. x \<le> N}"
+    and "i \<le> N"
+  shows "set (map (applySym2Form p) (formulasOverDownN2 N f i)) = set (formulasOverDownN2 N f (p i))"
+proof -
+  have a: "\<exists>x\<in>set (down N). applySym2Form p (f i j) = f (p i) x"
+    if "j \<in> set (down N)" for j
+  proof -
+    have a1: "j \<le> N"
+      using that set_down by auto 
+    show ?thesis
+      apply (rule bexI[where x="p j"])
+      using assms a1 unfolding symmetricParamFormulas2_def
+       apply simp
+      using a1 assms(2)
+      using permutes_in_image set_down by fastforce
+  qed
+  have b: "\<exists>x\<in>set (down N). f (p i) j = applySym2Form p (f i x)"
+    if "j \<in> set (down N)" for j
+  proof -
+    have b1: "j \<le> N"
+      using that set_down by auto
+    have b2: "j = p (inv p j)"
+      using assms(2) b1 permutes_inverses(1) by fastforce
+    have b3: "inv p j \<le> N"
+      using assms(2) b1
+      by (metis b2 mem_Collect_eq permutes_def)
+    show ?thesis
+      apply (rule bexI[where x="inv p j"])
+       apply (subst b2)
+      using assms b3 unfolding symmetricParamFormulas2_def
+      by (auto simp add: set_down)
+  qed
+  show ?thesis
+    unfolding formulasOverDownN2_def
+    apply (auto simp add: image_def)
+    using a b by auto
+qed
+
+
+subsection \<open>Strengthening\<close>
+
+text \<open>Next, consider the case of strengthening\<close>
+definition strengthenProt :: "nat \<Rightarrow> (nat \<Rightarrow> rule set) \<Rightarrow> (nat \<Rightarrow> nat \<Rightarrow> formula) \<Rightarrow> (nat \<Rightarrow> rule set)" where
+  "strengthenProt N rf invf i = (strengthenR1 (formulasOverDownN2 N invf i) []) ` (rf i)"
+
+lemma applySym2FormList:
+  "applySym2Form p (andList fs) = andList (map (applySym2Form p) fs)"
+  apply (induction fs)
+  by auto
+
+definition alphaEqRuleSet :: "rule set \<Rightarrow> rule set \<Rightarrow> bool" where
+  "alphaEqRuleSet rs1 rs2 \<longleftrightarrow>
+    (\<forall>r1\<in>rs1. \<exists>r2\<in>rs2. alphaEqRule r1 r2) \<and>
+    (\<forall>r2\<in>rs2. \<exists>r1\<in>rs1. alphaEqRule r1 r2)"
+
+definition symmetricParamRules' :: "nat \<Rightarrow> (nat \<Rightarrow> rule set) \<Rightarrow> bool" where [simp]:
+  "symmetricParamRules' N f = (\<forall>p i. p permutes {x. x \<le> N} \<longrightarrow> 
+i \<le> N \<longrightarrow> alphaEqRuleSet (applySym2Rule p ` f i) (f (p i)))"
+
+lemma alphaEqStrengthenR1:
+  assumes "applySym2Form p ` (set fs) = set fs2"
+  shows "alphaEqRule (applySym2Rule p (strengthenR1 fs [] r)) (strengthenR1 fs2 [] (applySym2Rule p r))"
+proof (cases r)
+  case (guard cond act)
+  have a: "and2ListF (applySym2Form p (andList fs)) = and2ListF (andList fs2)"
+    unfolding applySym2FormList
+    sorry
+  show ?thesis
+    unfolding guard apply simp
+    using a by auto
+qed
+
+lemma alphaEqStrengthenR1Set:
+  assumes "applySym2Form p ` (set fs) = set fs2"
+  shows "alphaEqRuleSet (applySym2Rule p ` strengthenR1 fs [] ` rs) (strengthenR1 fs2 [] ` applySym2Rule p ` rs)"
+proof -
+  have a: "\<exists>r2\<in>(strengthenR1 fs2 [] ` applySym2Rule p ` rs). (alphaEqRule r1 r2)"
+    if r1: "r1\<in>applySym2Rule p ` strengthenR1 fs [] ` rs" for r1
+  proof -
+    obtain r1' where r1': "r1' \<in> rs" "r1 = applySym2Rule p (strengthenR1 fs [] r1')"
+      using r1 by blast
+    show ?thesis
+      apply (rule bexI[where x="strengthenR1 fs2 [] (applySym2Rule p r1')"])
+      unfolding r1'(2)
+       apply (rule alphaEqStrengthenR1[OF assms])
+      using r1' by auto
+  qed
+  have b: "\<exists>r1\<in>applySym2Rule p ` strengthenR1 fs [] ` rs. alphaEqRule r1 r2"
+    if r2: "r2\<in>strengthenR1 fs2 [] ` applySym2Rule p ` rs" for r2
+  proof -
+    obtain r2' where r2': "r2' \<in> rs" "r2 = strengthenR1 fs2 [] (applySym2Rule p r2')"
+      using r2 by blast
+    show ?thesis
+      apply (rule bexI[where x="applySym2Rule p (strengthenR1 fs [] r2')"])
+      unfolding r2'(2)
+      apply (rule alphaEqStrengthenR1[OF assms])
+      using r2' by auto
+  qed
+  show ?thesis
+    unfolding alphaEqRuleSet_def
+    using a b by auto
+qed
+
+theorem strengthenProtSymmetric:
+  assumes "symmetricParamRules N rf"
+    and "symmetricParamFormulas2 N invf"
+  shows "symmetricParamRules' N (\<lambda>i. strengthenProt N rf invf i)"
+proof -
+  have a: "alphaEqRuleSet (applySym2Rule p ` strengthenProt N rf invf i) (strengthenProt N rf invf (p i))"
+    if "p permutes {x. x \<le> N}" "i \<le> N" for p i
+  proof -
+    from assms(1)[unfolded symmetricParamRules_def]
+    have a1: "applySym2Rule p ` rf i = rf (p i)"
+      using that by auto
+    show ?thesis
+      unfolding strengthenProt_def a1[symmetric]
+      apply (rule alphaEqStrengthenR1Set)
+      apply (subst image_set)
+      by (rule symParamFormulas[OF assms(2) that])
+  qed
+  show ?thesis
+    unfolding symmetricParamRules'_def
+    using a by auto
+qed
+
+theorem symProtFromSymmetricParam':
+  assumes "symmetricParamRules' N f"
+  shows "symProtRules' N (rulesOverDownN N f)"
+proof -
+  have a: "\<exists>r'. alphaEqRule r' (applySym2Rule p r) \<and> r' \<in> rulesOverDownN N f"
+    if aa: "p permutes {x. x \<le> N}" "r \<in> rulesOverDownN N f" for p r
+  proof -
+    obtain i where i: "i \<le> N" "r \<in> f i"
+      using aa(2) unfolding rulesOverDownN_def by auto 
+    from assms[unfolded symmetricParamRules'_def]
+    have a1: "alphaEqRuleSet (applySym2Rule p ` f i) (f (p i))"
+      using aa(1) i(1) by auto
+    have a2: "applySym2Rule p r \<in> applySym2Rule p ` f i"
+      using i(2) by auto
+    obtain r' where r': "r' \<in> f (p i)" "alphaEqRule (applySym2Rule p r) r'"
+      using a1 a2 unfolding alphaEqRuleSet_def by auto
+    have a3: "p i \<le> N"
+      using i(1) aa(1)
+      by (metis (full_types) mem_Collect_eq permutes_def)
+    show ?thesis
+      apply (rule exI[where x=r'])
+      using r' a3 by (auto simp add: rulesOverDownN_def)
+  qed
+  show ?thesis
+    unfolding symProtRules'_def
+    using a by auto
+qed
+
+end
