examples/n_german/german.thy
@@ -1,0 +1,191 @@
+theory german
+  imports Symmetric
+begin
+section{*Main definitions*}
+definition I::"scalrValueType" where [simp]: "I\<equiv> enum ''control'' ''I''"
+definition S::"scalrValueType" where [simp]: "S\<equiv> enum ''control'' ''S''"
+definition E::"scalrValueType" where [simp]: "E\<equiv> enum ''control'' ''E''"
+definition Empty::"scalrValueType" where [simp]: "Empty\<equiv> enum ''control'' ''Empty''"
+definition ReqS::"scalrValueType" where [simp]: "ReqS\<equiv> enum ''control'' ''ReqS''"
+definition ReqE::"scalrValueType" where [simp]: "ReqE\<equiv> enum ''control'' ''ReqE''"
+definition Inv::"scalrValueType" where [simp]: "Inv\<equiv> enum ''control'' ''Inv''"
+definition InvAck::"scalrValueType" where [simp]: "InvAck\<equiv> enum ''control'' ''InvAck''"
+definition GntS::"scalrValueType" where [simp]: "GntS\<equiv> enum ''control'' ''GntS''"
+definition GntE::"scalrValueType" where [simp]: "GntE\<equiv> enum ''control'' ''GntE''"
+definition true::"scalrValueType" where [simp]: "true\<equiv> boolV True"
+definition false::"scalrValueType" where [simp]: "false\<equiv> boolV False"
+
+definition n_RecvGntE1::"nat \<Rightarrow> rule" where [simp]:
+"n_RecvGntE1  i\<equiv>
+let g = (eqn (IVar (Para (''Chan2.Cmd'') i)) (Const GntE)) in
+
+let s = (parallelList [(assign ( (Para (''Cache.State'') i), (Const E))),
+ (assign ( (Para (''Cache.Data'') i), (IVar (Para (''Chan2.Data'') i)))),
+ (assign ( (Para (''Chan2.Cmd'') i), (Const Empty)))]) in
+guard g s"
+
+definition n_RecvGntS2::"nat \<Rightarrow> rule" where [simp]:
+"n_RecvGntS2  i\<equiv>
+let g = (eqn (Ivar (Para (''Chan2.Cmd'') i) (Const GntS))) in
+let s = (parallelList [(assign (Ivar (Para (''Cache.State'') i)
+(Const S))), (assign (Ivar (Para (''Cache.Data'') i), (IVar (Para (''Chan2.Data'') i))))
+ (assign (Ivar (Para (''Chan2.Cmd'') i), (Const Empty)))]) in
+guard g s"
+
+definition n_SendGntE3::"nat \<Rightarrow> rule" where [simp]:
+"n_SendGntE3  i\<equiv>
+let g = (andForm (eqn (IVar (Ident ''CurCmd'')) (Const ReqE)) (eqn (IVar (Ident ''CurPtr''))
+ (Const i)) (eqn (Ivar (Para (''Chan2.Cmd'') i) (Const Empty)))
+ (eqn (IVar (Ident ''ExGntd'')) (Const false)) 
+(forallForm (down N) (\<lambda>j. (eqn (Ivar (Para (''ShrSet'') j) (Const false))) ))in
+let s = (parallelList [(assign (Ivar (Para (''Chan2.Cmd'') i), (Const GntE))), 
+(assign (Ivar (Para (''Chan2.Data'') i),
+ (Const MemData))),
+ (assign (Ivar (Para (''ShrSet'') i), (Const true))),
+ (assign ((Ident ''ExGntd''), (Const true))),
+ (assign ((Ident ''CurCmd''), (Const Empty)))]) in
+guard g s"
+
+definition n_SendGntS4::"nat \<Rightarrow> rule" where [simp]:
+"n_SendGntS4  i\<equiv>
+let g = (andForm (eqn (IVar (Ident ''CurCmd'')) (Const ReqS)) (eqn (IVar (Ident ''CurPtr'')) (Const i)) (eqn (Ivar (Para (''Chan2.Cmd'') i) (Const Empty))) (eqn (IVar (Ident ''ExGntd'')) (Const false)) in
+let s = (parallelList [(assign (Ivar (Para (''Chan2.Cmd'') i), (Const GntS))), (assign (Ivar (Para (''Chan2.Data'') i), (Const MemData))), (assign (Ivar (Para (''ShrSet'') i), (Const true))), (assign ((Ident ''CurCmd''), (Const Empty)))]) in
+guard g s"
+
+definition n_RecvInvAck5::"nat \<Rightarrow> rule" where [simp]:
+"n_RecvInvAck5  i\<equiv>
+let g = (andForm (eqn (Ivar (Para (''Chan3.Cmd'') i) (Const InvAck))) (neg (eqn (IVar (Ident ''CurCmd'')) (Const Empty))) (eqn (IVar (Ident ''ExGntd'')) (Const true)) in
+let s = (parallelList [(assign (Ivar (Para (''Chan3.Cmd'') i), (Const Empty))), (assign (Ivar (Para (''ShrSet'') i), (Const false))), (assign ((Ident ''ExGntd''), (Const false))), (assign ((Ident ''MemData''), (IVar (Para (''Chan3.Data'') i))))]) in
+guard g s"
+
+definition n_RecvInvAck6::"nat \<Rightarrow> rule" where [simp]:
+"n_RecvInvAck6  i\<equiv>
+let g = (andForm (eqn (Ivar (Para (''Chan3.Cmd'') i) (Const InvAck))) (neg (eqn (IVar (Ident ''CurCmd'')) (Const Empty))) (neg (eqn (IVar (Ident ''ExGntd'')) (Const true))) in
+let s = (parallelList [(assign (Ivar (Para (''Chan3.Cmd'') i), (Const Empty))), (assign (Ivar (Para (''ShrSet'') i), (Const false)))]) in
+guard g s"
+
+definition n_SendInvAck7::"nat \<Rightarrow> rule" where [simp]:
+"n_SendInvAck7  i\<equiv>
+let g = (andForm (eqn (Ivar (Para (''Chan2.Cmd'') i) (Const Inv))) (eqn (Ivar (Para (''Chan3.Cmd'') i) (Const Empty))) (eqn (Ivar (Para (''Cache.State'') i) (Const E))) in
+let s = (parallelList [(assign (Ivar (Para (''Chan2.Cmd'') i), (Const Empty))), (assign (Ivar (Para (''Chan3.Cmd'') i), (Const InvAck))), (assign (Ivar (Para (''Chan3.Data'') i), (IVar (Para (''Cache.Data'') i)))), (assign (Ivar (Para (''Cache.State'') i), (Const I)))]) in
+guard g s"
+
+definition n_SendInvAck8::"nat \<Rightarrow> rule" where [simp]:
+"n_SendInvAck8  i\<equiv>
+let g = (andForm (eqn (Ivar (Para (''Chan2.Cmd'') i) (Const Inv))) (eqn (Ivar (Para (''Chan3.Cmd'') i) (Const Empty))) (neg (eqn (Ivar (Para (''Cache.State'') i) (Const E)))) in
+let s = (parallelList [(assign (Ivar (Para (''Chan2.Cmd'') i), (Const Empty))), (assign (Ivar (Para (''Chan3.Cmd'') i), (Const InvAck))), (assign (Ivar (Para (''Cache.State'') i), (Const I)))]) in
+guard g s"
+
+definition n_SendInv9::"nat \<Rightarrow> rule" where [simp]:
+"n_SendInv9  i\<equiv>
+let g = (andForm (eqn (Ivar (Para (''Chan2.Cmd'') i) (Const Empty))) (eqn (Ivar (Para (''InvSet'') i) (Const true))) (eqn (IVar (Ident ''CurCmd'')) (Const ReqE)) in
+let s = (parallelList [(assign (Ivar (Para (''Chan2.Cmd'') i), (Const Inv))), (assign (Ivar (Para (''InvSet'') i), (Const false)))]) in
+guard g s"
+
+definition n_SendInv10::"nat \<Rightarrow> rule" where [simp]:
+"n_SendInv10  i\<equiv>
+let g = (andForm (eqn (Ivar (Para (''Chan2.Cmd'') i) (Const Empty))) (eqn (Ivar (Para (''InvSet'') i) (Const true))) (eqn (IVar (Ident ''CurCmd'')) (Const ReqS)) (eqn (IVar (Ident ''ExGntd'')) (Const true)) in
+let s = (parallelList [(assign (Ivar (Para (''Chan2.Cmd'') i), (Const Inv))), (assign (Ivar (Para (''InvSet'') i), (Const false)))]) in
+guard g s"
+
+definition n_RecvReqE11::"nat \<Rightarrow> rule" where [simp]:
+"n_RecvReqE11  i\<equiv>
+let g = (andForm (eqn (IVar (Ident ''CurCmd'')) (Const Empty)) (eqn (Ivar (Para (''Chan1.Cmd'') i) (Const ReqE))) in
+let s = (parallelList [(assign ((Ident ''CurCmd''), (Const ReqE))), (assign ((Ident ''CurPtr''), (Const i))), (assign (Ivar (Para (''Chan1.Cmd'') i), (Const Empty))), (forallSent (down N) (\<lambda>j. (eqn (Ivar (Para (''InvSet'') j) (IVar (Para (''ShrSet'') j)))) ))]) in
+guard g s"
+
+definition n_RecvReqS12::"nat \<Rightarrow> rule" where [simp]:
+"n_RecvReqS12  i\<equiv>
+let g = (andForm (eqn (IVar (Ident ''CurCmd'')) (Const Empty)) (eqn (Ivar (Para (''Chan1.Cmd'') i) (Const ReqS))) in
+let s = (parallelList [(assign ((Ident ''CurCmd''), (Const ReqS))), (assign ((Ident ''CurPtr''), (Const i))), (assign (Ivar (Para (''Chan1.Cmd'') i), (Const Empty))), (forallSent (down N) (\<lambda>j. (eqn (Ivar (Para (''InvSet'') j) (IVar (Para (''ShrSet'') j)))) ))]) in
+guard g s"
+
+definition n_SendReqE13::"nat \<Rightarrow> rule" where [simp]:
+"n_SendReqE13  i\<equiv>
+let g = (andForm (eqn (Ivar (Para (''Chan1.Cmd'') i) (Const Empty))) (eqn (Ivar (Para (''Cache.State'') i) (Const I))) in
+let s = (parallelList [(assign (Ivar (Para (''Chan1.Cmd'') i), (Const ReqE)))]) in
+guard g s"
+
+definition n_SendReqE14::"nat \<Rightarrow> rule" where [simp]:
+"n_SendReqE14  i\<equiv>
+let g = (andForm (eqn (Ivar (Para (''Chan1.Cmd'') i) (Const Empty))) (eqn (Ivar (Para (''Cache.State'') i) (Const S))) in
+let s = (parallelList [(assign (Ivar (Para (''Chan1.Cmd'') i), (Const ReqE)))]) in
+guard g s"
+
+definition n_SendReqS15::"nat \<Rightarrow> rule" where [simp]:
+"n_SendReqS15  i\<equiv>
+let g = (andForm (eqn (Ivar (Para (''Chan1.Cmd'') i) (Const Empty))) (eqn (Ivar (Para (''Cache.State'') i) (Const I))) in
+let s = (parallelList [(assign (Ivar (Para (''Chan1.Cmd'') i), (Const ReqS)))]) in
+guard g s"
+
+definition n_Store16::"nat \<Rightarrow> rule" where [simp]:
+"n_Store16  i\<equiv>
+let g = (eqn (Ivar (Para (''Cache.State'') i) (Const E))) in
+let s = (parallelList [(assign (Ivar (Para (''Cache.Data'') i), (Const d))), (assign ((Ident ''AuxData''), (Const d)))]) in
+guard g s"
+
+definition rules::"nat \<Rightarrow> rule set" where [simp]:
+"rules N \<equiv> {r.
+(\<exists> i. i\<le>N\<and>r=n_RecvGntE1  i) \<or>
+(\<exists> i. i\<le>N\<and>r=n_RecvGntS2  i) \<or>
+(\<exists> i. i\<le>N\<and>r=n_SendGntE3  i) \<or>
+(\<exists> i. i\<le>N\<and>r=n_SendGntS4  i) \<or>
+(\<exists> i. i\<le>N\<and>r=n_RecvInvAck5  i) \<or>
+(\<exists> i. i\<le>N\<and>r=n_RecvInvAck6  i) \<or>
+(\<exists> i. i\<le>N\<and>r=n_SendInvAck7  i) \<or>
+(\<exists> i. i\<le>N\<and>r=n_SendInvAck8  i) \<or>
+(\<exists> i. i\<le>N\<and>r=n_SendInv9  i) \<or>
+(\<exists> i. i\<le>N\<and>r=n_SendInv10  i) \<or>
+(\<exists> i. i\<le>N\<and>r=n_RecvReqE11  i) \<or>
+(\<exists> i. i\<le>N\<and>r=n_RecvReqS12  i) \<or>
+(\<exists> i. i\<le>N\<and>r=n_SendReqE13  i) \<or>
+(\<exists> i. i\<le>N\<and>r=n_SendReqE14  i) \<or>
+(\<exists> i. i\<le>N\<and>r=n_SendReqS15  i) \<or>
+(\<exists> i. i\<le>N\<and>r=n_Store16  i)
+}"
+
+definition initSpec0::"nat \<Rightarrow> formula" where [simp]:
+"initSpec0 N (forallSent (down N) (\<lambda>i. (eqn (Ivar (Para (''Chan1.Cmd'') i) (Const Empty))) ))"
+
+definition initSpec1::"nat \<Rightarrow> formula" where [simp]:
+"initSpec1 N (forallSent (down N) (\<lambda>i. (eqn (Ivar (Para (''Chan2.Cmd'') i) (Const Empty))) ))"
+
+definition initSpec2::"nat \<Rightarrow> formula" where [simp]:
+"initSpec2 N (forallSent (down N) (\<lambda>i. (eqn (Ivar (Para (''Chan3.Cmd'') i) (Const Empty))) ))"
+
+definition initSpec3::"nat \<Rightarrow> formula" where [simp]:
+"initSpec3 N (forallSent (down N) (\<lambda>i. (eqn (Ivar (Para (''Cache.State'') i) (Const I))) ))"
+
+definition initSpec4::"nat \<Rightarrow> formula" where [simp]:
+"initSpec4 N (forallSent (down N) (\<lambda>i. (eqn (Ivar (Para (''InvSet'') i) (Const false))) ))"
+
+definition initSpec5::"nat \<Rightarrow> formula" where [simp]:
+"initSpec5 N (forallSent (down N) (\<lambda>i. (eqn (Ivar (Para (''ShrSet'') i) (Const false))) ))"
+
+definition initSpec6::"nat \<Rightarrow> formula" where [simp]:
+"initSpec6 N \<equiv> (eqn (IVar (Ident ''ExGntd'')) (Const false)) "
+
+definition initSpec7::"nat \<Rightarrow> formula" where [simp]:
+"initSpec7 N \<equiv> (eqn (IVar (Ident ''CurCmd'')) (Const Empty)) "
+
+definition initSpec8::"nat \<Rightarrow> formula" where [simp]:
+"initSpec8 N \<equiv> (eqn (IVar (Ident ''MemData'')) (Const d)) "
+
+definition initSpec9::"nat \<Rightarrow> formula" where [simp]:
+"initSpec9 N \<equiv> (eqn (IVar (Ident ''AuxData'')) (Const d)) "
+
+definition allInitSpecs::"nat \<Rightarrow> formula list" where [simp]:
+"allInitSpecs N \<equiv> [
+(initSpec0 N),
+(initSpec1 N),
+(initSpec2 N),
+(initSpec3 N),
+(initSpec4 N),
+(initSpec5 N),
+(initSpec6 N),
+(initSpec7 N),
+(initSpec8 N),
+(initSpec9 N)
+]"
+
+end
