examples/n_german/nMutualExBase2.thy
@@ -1,0 +1,249 @@
+theory nMutualExBase2
+  imports Symmetric
+begin
+
+text \<open>Represents four states: idle, try, critical, exit\<close>
+
+definition I :: scalrValueType where [simp]: "I \<equiv> enum ''control'' ''I''"
+definition T :: scalrValueType where [simp]: "T \<equiv> enum ''control'' ''T''"
+definition C :: scalrValueType where [simp]: "C \<equiv> enum ''control'' ''C''"
+definition E :: scalrValueType where [simp]: "E \<equiv> enum ''control'' ''E''"
+
+definition true :: scalrValueType where [simp]: "true \<equiv> boolV True"
+definition false :: scalrValueType where [simp]: "false \<equiv> boolV False"
+
+
+subsection \<open>Definitions of Parameterized Rules\<close>
+
+text \<open>If currently idle, can move to try
+  n[i] = I \<rightarrow> n[i] := T
+\<close>
+definition n_Try :: "nat \<Rightarrow> rule" where [simp]:
+  "n_Try i \<equiv>
+    let g = (eqn (IVar (Para ( ''n'') i)) (Const I)) in
+    let s = (parallelList [(assign ((Para ( ''n'') i), (Const T)))]) in
+      guard g s"
+
+text \<open>Enter critical region
+  n[i] = T \<and> x = True \<rightarrow> n[i] := C; x := False
+\<close>
+definition n_Crit :: "nat \<Rightarrow> rule" where [simp]:
+  "n_Crit i \<equiv>
+    let g = (andForm (eqn (IVar (Para ( ''n'') i)) (Const T)) (eqn (IVar (Ident ''x'')) (Const true))) in
+    let s = (parallelList [(assign ((Para ( ''n'') i), (Const C))), (assign ((Ident ''x''), (Const false)))]) in
+      guard g s"
+
+text \<open>Exit critical region
+  n[i] = C \<rightarrow> n[i] := E
+\<close>
+definition n_Exit::"nat \<Rightarrow> rule" where [simp]:
+  "n_Exit i \<equiv>
+    let g = (eqn (IVar (Para ( ''n'') i)) (Const C)) in
+    let s = (parallelList [(assign ((Para ( ''n'') i), (Const E)))]) in
+      guard g s"
+
+text \<open>Move to idle
+  n[i] = E \<rightarrow> n[i] := I; x := True
+\<close>
+definition n_Idle :: "nat \<Rightarrow> rule" where [simp]:
+  "n_Idle i \<equiv>
+    let g = (eqn (IVar (Para ( ''n'') i)) (Const E)) in
+    let s = (parallelList [(assign ((Para ( ''n'') i), (Const I))), (assign ((Ident ''x''), (Const true)))]) in
+      guard g s"
+
+
+definition rules :: "nat \<Rightarrow> rule set" where [simp]:
+  "rules N \<equiv> {r.
+    (\<exists>i. i \<le> N \<and> r = n_Try i) \<or>
+    (\<exists>i. i \<le> N \<and> r = n_Crit i) \<or>
+    (\<exists>i. i \<le> N \<and> r = n_Exit i) \<or>
+    (\<exists>i. i \<le> N \<and> r = n_Idle i) 
+   }"
+
+definition rules_i :: "nat \<Rightarrow> rule set" where
+  "rules_i i = {n_Try i, n_Crit i, n_Exit i, n_Idle i}"
+
+lemma rules_i_same:
+  "rulesOverDownN N (rules_i) = rules N"
+  unfolding rules_def rules_i_def rulesOverDownN_def
+  by auto
+
+lemma rule_i_symmetric:
+  "symmetricParamRules N rules_i"
+  unfolding symmetricParamRules_def rules_i_def
+  by auto
+
+theorem rulesSymmetric:
+  "symProtRules N (rules N)"
+  unfolding rules_i_same[symmetric]
+  apply (rule symProtFromSymmetricParam)
+  by (rule rule_i_symmetric)
+
+lemma rule_i_symmetric':
+  "symmetricParamRules' N rules_i"
+  unfolding symmetricParamRules'_def rules_i_def
+  
+  using alphaEqRuleSet_def by auto
+
+text \<open>No two processes can be in the exit state in the same time.
+  i \<noteq> j \<longrightarrow> n[i] = E \<longrightarrow> n[j] \<noteq> E
+\<close>
+definition inv_7 :: "nat \<Rightarrow> nat \<Rightarrow> formula" where [simp]:
+  "inv_7 i j \<equiv>
+    implyForm (andForm (neg (eqn (Const (index i)) (Const (index j)))) (eqn (IVar (Para ''n'' i)) (Const E))) 
+      (neg (eqn (IVar (Para ''n'' j)) (Const E)))"
+
+text \<open>There cannot be one state in exit and another in critical.
+  i \<noteq> j \<longrightarrow> n[i] = E \<longrightarrow> n[j] \<noteq> C
+\<close>
+definition inv_5 :: "nat \<Rightarrow> nat \<Rightarrow> formula" where [simp]:
+  "inv_5 i j \<equiv>
+    implyForm (andForm (neg (eqn (Const (index i)) (Const (index j))))  
+      (eqn (IVar (Para ''n'' i)) (Const E))) (neg (eqn (IVar (Para ''n'' j)) (Const C)))"
+
+definition inv_57 :: "nat \<Rightarrow> nat \<Rightarrow> formula" where
+  "inv_57 i j = andForm (inv_5 i j) (inv_7 i j)"
+
+lemma inv_57_symmetric2:
+  "symmetricParamFormulas2 N inv_57"
+  unfolding symmetricParamFormulas2_def inv_57_def by auto
+
+subsection \<open>Strengthened rules\<close>
+
+definition rules2 :: "nat \<Rightarrow> rule set" where
+  "rules2 N = rulesOverDownN N (\<lambda>i. strengthenProt N rules_i inv_57 i)"
+
+theorem rules2_symmetric:
+  "symProtRules' N (rules2 N)"
+  unfolding rules2_def
+  apply (rule symProtFromSymmetricParam')
+  apply (rule strengthenProtSymmetric)
+   apply (rule rule_i_symmetric)
+  by (rule inv_57_symmetric2)
+
+(*definition I::"scalrValueType" where [simp]: "I\<equiv> enum ''control1'' ''I''"*)
+definition S::"scalrValueType" where [simp]: "S\<equiv> enum ''control'' ''S''"
+(*definition E::"scalrValueType" where [simp]: "E\<equiv> enum ''control1'' ''E''"*)
+definition Empty::"scalrValueType" where [simp]: "Empty\<equiv> enum ''control'' ''Empty''"
+definition ReqS::"scalrValueType" where [simp]: "ReqS\<equiv> enum ''control'' ''ReqS''"
+definition ReqE::"scalrValueType" where [simp]: "ReqE\<equiv> enum ''control'' ''ReqE''"
+definition Inv::"scalrValueType" where [simp]: "Inv\<equiv> enum ''control'' ''Inv''"
+definition InvAck::"scalrValueType" where [simp]: "InvAck\<equiv> enum ''control'' ''InvAck''"
+definition GntS::"scalrValueType" where [simp]: "GntS\<equiv> enum ''control'' ''GntS''"
+definition GntE::"scalrValueType" where [simp]: "GntE\<equiv> enum ''control'' ''GntE''" 
+
+definition n_SendReqS15::"nat \<Rightarrow> rule" where [simp]:
+"n_SendReqS15  i\<equiv>
+let g = (andForm (eqn (IVar (Para (''Chan1.Cmd'') i)) (Const Empty))
+   (eqn (IVar (Para (''Cache.State'') i)) (Const I))) in
+let s = (parallelList [(assign ( (Para (''Chan1.Cmd'') i), (Const ReqS)))]) in
+guard g s"
+
+
+definition n_SendGntE3::"nat\<Rightarrow> nat\<Rightarrow> rule" where [simp]:
+"n_SendGntE3 N  i\<equiv>
+let g = andList [ (eqn (IVar (Ident ''CurCmd'')) (Const ReqE)),
+ (eqn (IVar (Ident ''CurPtr''))(Const (index i))),
+ (eqn (IVar (Para (''Chan2.Cmd'') i)) (Const Empty)),
+ (eqn (IVar (Ident ''ExGntd'')) (Const false)), 
+  andList (map  (\<lambda>j. (eqn (IVar (Para (''ShrSet'') j)) (Const false))) (down N)) 
+] in
+let s = (parallelList [assign  ((Para (''Chan2.Cmd'') i), (Const GntE)), 
+assign ( (Para (''Chan2.Data'') i),(IVar (Ident ''MemData''))),
+assign ( (Para (''ShrSet'') i), (Const true)),
+assign ((Ident ''ExGntd''), (Const true)),
+assign ((Ident ''CurCmd''), (Const Empty))]) in
+guard g s"
+
+(*(forallForm (down N) (\<lambda>j. (eqn (IVar (Para (''ShrSet'') j)) (Const false))) )*)
+definition rules_i1 :: "nat\<Rightarrow>nat \<Rightarrow> rule set" where
+  "rules_i1 N i = {n_Try i, n_Crit i, n_Exit i, n_Idle i,n_SendReqS15  i,n_SendGntE3 N  i}"
+
+(*lemma rules_i_same:
+  "rulesOverDownN N (rules_i) = rules N"
+  unfolding rules_def rules_i_def rulesOverDownN_def
+  by auto
+*)
+
+(*lemma andListSym:
+  assumes a1:"\<forall>f. f \<in>set fl \<longrightarrow> (\<exists>f'. f'\<in>set fl' \<longrightarrow>alphaEqForm (applySym2Form p f)  f') " and
+  a2:"\<forall>f'. f' \<in>set fl' \<longrightarrow> (\<exists>f. f\<in>set fl \<longrightarrow>alphaEqForm (applySym2Form p f)  f')"
+  and a3:"p permutes {x. x \<le> N}"
+  shows "alphaEqForm (applySym2Form p (andList fl)) (andList fl') "
+  sorry 
+*)
+(*
+(forallForm (down N) (\<lambda>j. (eqn (IVar (Para (''ShrSet'') j)) (Const false))) ))
+   
+  (forallForm (down N) (\<lambda>j. (eqn (IVar (Para (''ShrSet'') j)) (Const false))) )*)
+
+lemma for1:assumes  a2:"p permutes {x. x \<le> N}"
+  shows
+  "and2ListF 
+  (andList (map  (\<lambda>j. (eqn (IVar (Para (''ShrSet'') j)) (Const false))) (down N))) =
+  and2ListF (applySym2Form p  
+  (andList (map  (\<lambda>j. (eqn (IVar (Para (''ShrSet'') j)) (Const false))) (down N))))"
+  (is "?P (applySym2Form p  (andList ?fl)) (andList ?fl')") 
+  apply(rule wellFormAndlistIsSym1)
+   apply auto
+  by(cut_tac a2,auto)
+(*  by (metis alphaEqForm_def andListApplySym0 andListSym empty_iff list.set(1) permutes_def) 
+proof(rule andListSym)
+  show "\<forall>f. f \<in>set ?fl \<longrightarrow> (\<exists>f'. f'\<in>set ?fl' \<longrightarrow>alphaEqForm (applySym2Form p f)  f') "
+    using alphaEqForm_def by blast
+next
+  show "\<forall>f'. f' \<in>set ?fl' \<longrightarrow> (\<exists>f. f\<in>set ?fl \<longrightarrow>alphaEqForm (applySym2Form p f)  f')"
+    sorry
+next
+  show "p permutes {x. x \<le> N}"
+    using assms by blast
+  
+qed*)
+
+lemma r1:
+  assumes  a2:"p permutes {x. x \<le> N}"
+  shows a1:"alphaEqForm   (applySym2Form p (pre(n_SendGntE3 N  i))) (pre(n_SendGntE3 N  (p i)))"
+proof -
+  have a1:"and2ListF 
+  (andList (map  (\<lambda>j. (eqn (IVar (Para (''ShrSet'') j)) (Const false))) (down N))) =
+  and2ListF (applySym2Form p  
+  (andList (map  (\<lambda>j. (eqn (IVar (Para (''ShrSet'') j)) (Const false))) (down N))))"
+    using assms for1 by auto
+  show "alphaEqForm (applySym2Form p (pre (n_SendGntE3 N i))) (pre (n_SendGntE3 N (p i))) " 
+    apply(simp,auto)
+    apply(cut_tac  a1)  
+     apply force
+    apply(cut_tac  a1)  
+    apply force
+   done
+qed
+ (* apply(simp,auto)
+   apply(cut_tac for1 a2)  
+    apply force
+  
+   apply(cut_tac for1 a2)  
+  apply force
+  apply (metis (no_types, lifting) Collect_cong alphaEqForm_def andListSym applySym2FormList assms empty_iff list.set(1) map_map onMapAndListF)
+  apply (metis (no_types, lifting) Collect_cong alphaEqForm_def andListSym applySym2FormList assms empty_iff list.set(1) map_map onMapAndListF)
+  done*)
+
+  (*using andListSym apply force
+  apply(simp del:andCons alphaEqForm_def)
+  apply(rule andListSym)
+   apply (metis (mono_tags, hide_lams) a1 a2 alphaEqForm_def andListForm2 andListForm3 andListSym empty_iff formEval.simps(3) insert_iff list.set(1) list.set(2)
+ list.set_intros(1) stFormSymCorrespondence)
+  apply(rule allI,auto)
+  using andListSym for1 apply force
+  
+  using andListSym apply force
+  done*)
+  
+
+lemma rule_i1_symmetric:
+  "symmetricParamRules' N (rules_i1 N)"
+  unfolding symmetricParamRules'_def rules_i1_def
+  using r1 alphaEqRuleSet_def by auto
+  
+
+
+end
